MPL/ProofMode.lean
@@ -1,3 +1,3 @@
-import MPL.ProofMode.SGoal
+import MPL.ProofMode.MGoal
 import MPL.ProofMode.Tactics
 import MPL.ProofMode.Display
