MPL/ProofMode/Patterns/MCases.lean
@@ -1,0 +1,50 @@
+/-
+Copyright (c) 2022 Lars König. All rights reserved.
+Released under Apache 2.0 license as described in the file LICENSE.
+Authors: Lars König
+-/
+import Lean.Data.Name
+
+namespace MPL.ProofMode.Patterns
+open Lean
+
+declare_syntax_cat mcasesPat
+syntax mcasesPatAlts := sepBy1(mcasesPat, " | ")
+syntax binderIdent : mcasesPat
+syntax "-" : mcasesPat
+syntax "⟨" mcasesPatAlts,* "⟩" : mcasesPat
+syntax "(" mcasesPatAlts ")" : mcasesPat
+syntax "⌜" binderIdent "⌝" : mcasesPat
+syntax "□" binderIdent : mcasesPat
+
+macro "%" h:binderIdent : mcasesPat => `(mcasesPat| ⌜$h⌝)
+macro "#" h:binderIdent : mcasesPat => `(mcasesPat| □ $h)
+
+inductive MCasesPat
+  | one (name : TSyntax ``binderIdent)
+  | clear
+  | tuple (args : List MCasesPat)
+  | alts (args : List MCasesPat)
+  | pure       (h : TSyntax ``binderIdent)
+  | stateful (h : TSyntax ``binderIdent)
+  deriving Repr, Inhabited
+
+partial def MCasesPat.parse (pat : TSyntax `mcasesPat) : MacroM MCasesPat := do
+  match go ⟨← expandMacros pat⟩ with
+  | none => Macro.throwUnsupported
+  | some pat => return pat
+where
+  go : TSyntax `mcasesPat → Option MCasesPat
+  | `(mcasesPat| $name:binderIdent) => some <| .one name
+  | `(mcasesPat| -) => some <| .clear
+  | `(mcasesPat| ⟨$[$args],*⟩) => args.mapM goAlts |>.map (.tuple ·.toList)
+  | `(mcasesPat| ⌜$h⌝) => some (.pure h)
+  | `(mcasesPat| □$h) => some (.stateful h)
+  | `(mcasesPat| ($pat)) => goAlts pat
+  | _ => none
+  goAlts : TSyntax ``mcasesPatAlts → Option MCasesPat
+  | `(mcasesPatAlts| $args|*) =>
+    match args.getElems with
+    | #[arg] => go arg
+    | args   => args.mapM go |>.map (.alts ·.toList)
+  | _ => none
