MPL/ProofMode/Tactics/Clear.lean
@@ -3,24 +3,24 @@ Copyright (c) 2022 Lars König. All rights reserved.
 Released under Apache 2.0 license as described in the file LICENSE.
 Authors: Lars König, Mario Carneiro
 -/
-import MPL.ProofMode.SGoal
+import MPL.ProofMode.MGoal
 import MPL.ProofMode.Focus
 
 namespace MPL.ProofMode.Tactics
 open Lean Elab Tactic Meta
 
-theorem clear {σs : List Type} {P P' A Q : SPred σs}
+theorem Clear.clear {σs : List Type} {P P' A Q : SPred σs}
     (hfocus : P ⊣⊢ₛ P' ∧ A) (h : P' ⊢ₛ Q) : P ⊢ₛ Q :=
     hfocus.mp.trans <| (SPred.and_mono_l h).trans SPred.and_elim_l
 
-elab "sclear" colGt hyp:ident : tactic => do
+elab "mclear" colGt hyp:ident : tactic => do
   let mvar ← getMainGoal
   mvar.withContext do
   let g ← instantiateMVars <| ← mvar.getType
-  let some goal := parseSGoal? g | throwError "not in proof mode"
+  let some goal := parseMGoal? g | throwError "not in proof mode"
   let some res := goal.focusHyp hyp.getId | throwError "unknown identifier '{hyp}'"
   let m ← mkFreshExprSyntheticOpaqueMVar (res.restGoal goal).toExpr
 
-  mvar.assign (mkApp7 (mkConst ``clear) goal.σs goal.hyps
+  mvar.assign (mkApp7 (mkConst ``Clear.clear) goal.σs goal.hyps
     res.restHyps res.focusHyp goal.target res.proof m)
   replaceMainGoal [m.mvarId!]
