MPL/ProofMode/Tactics/Exact.lean
@@ -10,7 +10,7 @@ theorem Exact.assumption {σs : List Type} {P P' A : SPred σs}
 theorem Exact.from_tautology {σs : List Type} {P T : SPred σs} (htaut : ⊢ₛ T) : P ⊢ₛ T :=
   SPred.true_intro.trans htaut
 
-def _root_.MPL.ProofMode.SGoal.exact (goal : SGoal) (hyp : TSyntax `term) : OptionT MetaM Expr := do
+def _root_.MPL.ProofMode.MGoal.exact (goal : MGoal) (hyp : TSyntax `term) : OptionT MetaM Expr := do
   let some focusRes := goal.focusHyp hyp.raw.getId | failure
   OptionT.mk do
   let proof := mkApp5 (mkConst ``Exact.assumption) goal.σs goal.hyps focusRes.restHyps goal.target focusRes.proof
@@ -18,7 +18,7 @@ def _root_.MPL.ProofMode.SGoal.exact (goal : SGoal) (hyp : TSyntax `term) : Opti
     throwError "sexact tactic failed, hypothesis {hyp} is not definitionally equal to {goal.target}"
   return proof
 
-def _root_.MPL.ProofMode.SGoal.exactPure (goal : SGoal) (hyp : TSyntax `term) : TacticM Expr := do
+def _root_.MPL.ProofMode.MGoal.exactPure (goal : MGoal) (hyp : TSyntax `term) : TacticM Expr := do
   let T := goal.target
   let expected := mkApp2 (mkConst ``SPred.tautological) goal.σs T
   let prf ← try
@@ -26,11 +26,11 @@ def _root_.MPL.ProofMode.SGoal.exactPure (goal : SGoal) (hyp : TSyntax `term) : 
   catch _ => throwError "sexact tactic failed, {hyp} does not have type {expected}"
   return mkApp4 (mkConst ``Exact.from_tautology) goal.σs goal.hyps goal.target prf
 
-elab "sexact" colGt hyp:term : tactic => do
+elab "mexact" colGt hyp:term : tactic => do
   let mvar ← getMainGoal
   mvar.withContext do
   let g ← instantiateMVars <| ← mvar.getType
-  let some goal := parseSGoal? g | throwError "not in proof mode"
+  let some goal := parseMGoal? g | throwError "not in proof mode"
   if let some prf ← liftMetaM (goal.exact hyp) then
     mvar.assign prf
   else
