MPL/ProofMode/Tactics/Refine.lean
@@ -1,5 +1,5 @@
 import MPL.ProofMode.Focus
-import MPL.ProofMode.Patterns.SRefine
+import MPL.ProofMode.Patterns.MRefine
 import MPL.ProofMode.Tactics.Assumption
 import MPL.ProofMode.Tactics.Exact
 
@@ -7,7 +7,7 @@ namespace MPL.ProofMode.Tactics
 open MPL.ProofMode.Patterns
 open Lean Elab Tactic Meta
 
-def patAsTerm (pat : SRefinePat) (expected : Option Expr := none) : OptionT TacticM Expr := do
+def patAsTerm (pat : MRefinePat) (expected : Option Expr := none) : OptionT TacticM Expr := do
   match pat with
   | .pure t => elabTerm t expected
   | .one name =>
@@ -16,7 +16,7 @@ def patAsTerm (pat : SRefinePat) (expected : Option Expr := none) : OptionT Tact
     else failure
   | _ => failure
 
-partial def sRefineCore (goal : SGoal) (pat : SRefinePat) (k : SGoal → TSyntax ``binderIdent → TacticM Expr) : TacticM Expr := do
+partial def mRefineCore (goal : MGoal) (pat : MRefinePat) (k : MGoal → TSyntax ``binderIdent → TacticM Expr) : TacticM Expr := do
   match pat with
   | .stateful name => liftMetaM do
     match name with
@@ -30,39 +30,39 @@ partial def sRefineCore (goal : SGoal) (pat : SRefinePat) (k : SGoal → TSyntax
     goal.exactPure t
   | .one name =>
       if let `(binderIdent| $id:ident) := name then
-        sRefineCore goal (.pure (← `($id))) k <|> sRefineCore goal (.stateful name) k
+        mRefineCore goal (.pure (← `($id))) k <|> mRefineCore goal (.stateful name) k
       else
-        sRefineCore goal (.stateful name) k
+        mRefineCore goal (.stateful name) k
   | .hole name => k goal name
   | .tuple [] => throwUnsupportedSyntax
-  | .tuple [p] => sRefineCore goal p k
+  | .tuple [p] => mRefineCore goal p k
   | .tuple (p::ps) => do
-    let T := goal.target
+    let T ← whnfR goal.target
     if let some (σs, T₁, T₂) := parseAnd? T.consumeMData then
-      let prf₁ ← sRefineCore { goal with target := T₁ } p k
-      let prf₂ ← sRefineCore { goal with target := T₂ } (.tuple ps) k
+      let prf₁ ← mRefineCore { goal with target := T₁ } p k
+      let prf₂ ← mRefineCore { goal with target := T₂ } (.tuple ps) k
       return mkApp6 (mkConst ``SPred.and_intro) σs goal.hyps T₁ T₂ prf₁ prf₂
     else if let some (α, σs, ψ) := T.app3? ``SPred.exists then
       let some witness ← patAsTerm p (some α) | throwError "pattern does not elaborate to a term to instantiate ψ"
-      let prf ← sRefineCore { goal with target := ψ.betaRev #[witness] } (.tuple ps) k
+      let prf ← mRefineCore { goal with target := ψ.betaRev #[witness] } (.tuple ps) k
       let u ← getLevel α
       return mkApp6 (mkConst ``SPred.exists_intro' [u]) α σs goal.hyps ψ witness prf
     else throwError "Neither a conjunction nor an existential quantifier {goal.target}"
 
-elab "srefine" pat:srefinePat : tactic => do
-  let pat ← liftMacroM <| SRefinePat.parse pat
-  let (mvar, goal) ← sstart (← getMainGoal)
+elab "mrefine" pat:mrefinePat : tactic => do
+  let pat ← liftMacroM <| MRefinePat.parse pat
+  let (mvar, goal) ← mStart (← getMainGoal)
   mvar.withContext do
 
   let goals ← IO.mkRef #[]
-  let prf ← sRefineCore goal pat fun goal name => do
+  let prf ← mRefineCore goal pat fun goal name => do
     let m ← mkFreshExprSyntheticOpaqueMVar goal.toExpr name.raw.getId
     goals.modify (·.push m.mvarId!)
     return m
   mvar.assign prf
   replaceMainGoal (← goals.get).toList
 
-macro "sexists" args:term,+ : tactic => do
-  let pats ← args.getElems.mapM fun t => `(srefinePat| ⌜$t⌝)
-  let pat ← pats.foldrM (fun pat acc => `(srefinePat| ⟨$pat, $acc⟩)) (← `(srefinePat| ?_))
-  `(tactic| (srefine $pat; try sassumption))
+macro "mexists" args:term,+ : tactic => do
+  let pats ← args.getElems.mapM fun t => `(mrefinePat| ⌜$t⌝)
+  let pat ← pats.foldrM (fun pat acc => `(mrefinePat| ⟨$pat, $acc⟩)) (← `(mrefinePat| ?_))
+  `(tactic| (mrefine $pat; try massumption))
