MPL/ProofMode/Tactics/Specialize.lean
@@ -1,4 +1,4 @@
-import MPL.ProofMode.SGoal
+import MPL.ProofMode.MGoal
 import MPL.ProofMode.Focus
 import MPL.ProofMode.Tactics.Basic
 
@@ -8,7 +8,7 @@ open Lean Elab Tactic Meta
 
 initialize registerTraceClass `mpl.tactics.specialize
 
-theorem specialize_imp_stateful {P P' Q R : SPred σs}
+theorem Specialize.imp_stateful {P P' Q R : SPred σs}
   (hrefocus : P ∧ (Q → R) ⊣⊢ₛ P' ∧ Q) : P ∧ (Q → R) ⊢ₛ P ∧ R := by
   calc spred(P ∧ (Q → R))
     _ ⊢ₛ (P' ∧ Q) ∧ (Q → R) := SPred.and_intro hrefocus.mp SPred.and_elim_r
@@ -17,16 +17,16 @@ theorem specialize_imp_stateful {P P' Q R : SPred σs}
     _ ⊢ₛ (P' ∧ Q) ∧ R := SPred.and_assoc.mpr
     _ ⊢ₛ P ∧ R := SPred.and_mono_l (hrefocus.mpr.trans SPred.and_elim_l)
 
-theorem specialize_imp_pure {P Q R : SPred σs}
+theorem Specialize.imp_pure {P Q R : SPred σs}
   (h : ⊢ₛ Q) : P ∧ (Q → R) ⊢ₛ P ∧ R := by
   calc spred(P ∧ (Q → R))
     _ ⊢ₛ P ∧ (Q ∧ (Q → R)) := SPred.and_mono_r (SPred.and_intro (SPred.true_intro.trans h) .rfl)
     _ ⊢ₛ P ∧ R := SPred.and_mono_r (SPred.mp SPred.and_elim_r SPred.and_elim_l)
 
-theorem specialize_forall {P : SPred σs} {ψ : α → SPred σs}
+theorem Specialize.forall {P : SPred σs} {ψ : α → SPred σs}
   (a : α) : P ∧ (∀ x, ψ x) ⊢ₛ P ∧ ψ a := SPred.and_mono_r (SPred.forall_elim a)
 
-def specializeImpStateful (σs : Expr) (P : Expr) (QR : Expr) (arg : TSyntax `term) : OptionT TacticM (Expr × Expr) := do
+def mSpecializeImpStateful (σs : Expr) (P : Expr) (QR : Expr) (arg : TSyntax `term) : OptionT TacticM (Expr × Expr) := do
   guard (arg.raw.isIdent)
   let some arg := focusHyp σs (mkAnd! σs P QR) arg.raw.getId | failure
   OptionT.mk do -- no OptionT failure after this point
@@ -38,7 +38,7 @@ def specializeImpStateful (σs : Expr) (P : Expr) (QR : Expr) (arg : TSyntax `te
   let Q := arg.focusHyp
   let hrefocus := arg.proof -- P ∧ (Q → R) ⊣⊢ₛ P' ∧ Q
   let mkApp3 (.const ``SPred.imp []) σs Q' R := specHyp.p | throwError "Expected implication {QR}"
-  let proof := mkApp6 (mkConst ``specialize_imp_stateful) σs P P' Q R hrefocus
+  let proof := mkApp6 (mkConst ``Specialize.imp_stateful) σs P P' Q R hrefocus
   -- check proof
   trace[mpl.tactics.specialize] "Statefully specialize {specHyp.p} with {Q}. New Goal: {mkAnd! σs P R}"
   unless ← isDefEq Q Q' do
@@ -46,7 +46,7 @@ def specializeImpStateful (σs : Expr) (P : Expr) (QR : Expr) (arg : TSyntax `te
 
   return ({ specHyp with p := R }.toExpr, proof)
 
-def specializeImpPure (_σs : Expr) (P : Expr) (QR : Expr) (arg : TSyntax `term) : OptionT TacticM (Expr × Expr) := do
+def mSpecializeImpPure (_σs : Expr) (P : Expr) (QR : Expr) (arg : TSyntax `term) : OptionT TacticM (Expr × Expr) := do
   let some specHyp := parseHyp? QR | panic! "Precondition of specializeImpPure violated"
   let mkApp3 (.const ``SPred.imp []) σs Q R := specHyp.p | failure
   let (hQ, mvarIds) ← try
@@ -56,13 +56,13 @@ def specializeImpPure (_σs : Expr) (P : Expr) (QR : Expr) (arg : TSyntax `term)
   -- The goal is P ∧ (Q → R)
   -- we want to return (R, (proof : P ∧ (Q → R) ⊢ₛ P ∧ R))
   pushGoals mvarIds
-  let proof := mkApp5 (mkConst ``specialize_imp_pure) σs P Q R hQ
+  let proof := mkApp5 (mkConst ``Specialize.imp_pure) σs P Q R hQ
   -- check proof
   trace[mpl.tactics.specialize] "Purely specialize {specHyp.p} with {Q}. New Goal: {mkAnd! σs P R}"
   -- logInfo m!"proof: {← inferType proof}"
   return ({ specHyp with p := R }.toExpr, proof)
 
-def specializeForall (_σs : Expr) (P : Expr) (Ψ : Expr) (arg : TSyntax `term) : OptionT TacticM (Expr × Expr) := do
+def mSpecializeForall (_σs : Expr) (P : Expr) (Ψ : Expr) (arg : TSyntax `term) : OptionT TacticM (Expr × Expr) := do
   let some specHyp := parseHyp? Ψ | panic! "Precondition of specializeForall violated"
   let mkApp3 (.const ``SPred.forall [u]) α σs αR := specHyp.p | failure
   let (a, mvarIds) ← try
@@ -70,7 +70,7 @@ def specializeForall (_σs : Expr) (P : Expr) (Ψ : Expr) (arg : TSyntax `term) 
     catch _ => failure
   OptionT.mk do -- no OptionT failure after this point
   pushGoals mvarIds
-  let proof := mkApp5 (mkConst ``specialize_forall [u]) σs α P αR a
+  let proof := mkApp5 (mkConst ``Specialize.forall [u]) σs α P αR a
   let R := αR.beta #[a]
   -- check proof
   trace[mpl.tactics.specialize] "Instantiate {specHyp.p} with {a}. New Goal: {mkAnd! σs P R}"
@@ -79,8 +79,8 @@ def specializeForall (_σs : Expr) (P : Expr) (Ψ : Expr) (arg : TSyntax `term) 
 theorem focus {P P' Q R : SPred σs} (hfocus : P ⊣⊢ₛ P' ∧ Q) (hnew : P' ∧ Q ⊢ₛ R) : P ⊢ₛ R :=
   hfocus.mp.trans hnew
 
-elab "sspecialize" hyp:ident args:(colGt term:max)* : tactic => do
-  let (mvar, goal) ← sstart (← getMainGoal)
+elab "mspecialize" hyp:ident args:(colGt term:max)* : tactic => do
+  let (mvar, goal) ← mStart (← getMainGoal)
   mvar.withContext do
 
   -- Want to prove goal P ⊢ T, where hyp occurs in P.
@@ -95,16 +95,16 @@ elab "sspecialize" hyp:ident args:(colGt term:max)* : tactic => do
   let σs := goal.σs
   let P := specFocus.restHyps
   let mut H := specFocus.focusHyp
-  let mut goal : SGoal := goal
+  let mut goal : MGoal := goal
   -- invariant: proof (_ : goal.toExpr) fills the mvar
   let mut proof : Expr → Expr :=
     mkApp7 (mkConst ``focus) σs goal.hyps P H goal.target specFocus.proof
 
   for arg in args do
     let res? ← OptionT.run
-      (specializeImpStateful σs P H arg
-        <|> specializeImpPure σs P H arg
-        <|> specializeForall σs P H arg)
+      (mSpecializeImpStateful σs P H arg
+        <|> mSpecializeImpPure σs P H arg
+        <|> mSpecializeForall σs P H arg)
     match res? with
     | some (H', H2H') =>
       -- logInfo m!"H: {H}, proof: {← inferType H2H'}"
